fixed bug in alloc.bpl with respect to permission creation in atomic actions

Test/civl/alloc.bpl
@@ -7,14 +7,15 @@ function {:linear "mem"} dom(lmap): [int]bool;
 function map(lmap): [int]int;
 function cons([int]bool, [int]int) : lmap;
 axiom (forall x: [int]bool, y: [int]int :: {cons(x,y)} dom(cons(x, y)) == x && map(cons(x,y)) == y);
+axiom (forall x: lmap :: {dom(x)} {map(x)} cons(dom(x), map(x)) == x);
 
-function EmptyLmap(): (lmap);
-axiom (dom(EmptyLmap()) == MapConstBool(false));
+function Empty(m:[int]int): lmap;
+axiom (forall m: [int]int :: Empty(m) == cons(MapConstBool(false), m));
 
-function Add(x: lmap, i: int): (lmap);
+function Add(x: lmap, i: int): lmap;
 axiom (forall x: lmap, i: int :: dom(Add(x, i)) == dom(x)[i:=true] && map(Add(x, i)) == map(x));
 
-function Remove(x: lmap, i: int): (lmap);
+function Remove(x: lmap, i: int): lmap;
 axiom (forall x: lmap, i: int :: dom(Remove(x, i)) == dom(x)[i:=false] && map(Remove(x, i)) == map(x));
 
 function {:inline} PoolInv(unallocated:[int]bool, pool: lmap) : (bool)
@@ -76,7 +77,7 @@ procedure {:yields} {:layer 1,2} Alloc() returns ({:layer 1} {:linear "mem"} l: 
 requires {:layer 1} PoolInv(unallocated, pool);
 ensures  {:layer 1} PoolInv(unallocated, pool);
 ensures  {:layer 1} dom(l)[i] && map(l)[i] == mem[i];
-ensures {:right} |{ A: assume dom(l)[i]; return true; }|;
+ensures {:right} |{ var m:[int]int; A: assume dom(pool)[i]; pool := Remove(pool, i); l := Add(Empty(m), i); return true; }|;
 {
     call Yield();
     call i := PickAddr();
@@ -88,7 +89,7 @@ procedure {:yields} {:layer 1,2} Free({:layer 1} {:linear_in "mem"} l: lmap, i: 
 requires {:layer 1} PoolInv(unallocated, pool);
 ensures  {:layer 1} PoolInv(unallocated, pool);
 requires {:layer 1} dom(l)[i];
-ensures {:both} |{ A: return true; }|;
+ensures {:left} |{ A: assert dom(l)[i]; pool := Add(pool, i); return true; }|;
 {
     call Yield();
     call FreeLinear(l, i);
@@ -123,7 +124,7 @@ ensures {:both} |{ A: assert dom(l)[i]; l' := cons(dom(l), map(l)[i := o]); retu
 procedure {:layer 1} AllocLinear(i: int) returns ({:linear "mem"} l: lmap);
 modifies pool;
 requires dom(pool)[i];
-ensures pool == Remove(old(pool), i) && dom(l)[i] && map(l)[i] == mem[i];
+ensures pool == Remove(old(pool), i) && l == Add(Empty(mem), i);
 
 procedure {:layer 1} FreeLinear({:linear_in "mem"} l: lmap, i: int);
 modifies pool;
@@ -158,7 +159,7 @@ procedure {:yields} {:layer 2} Dummy()
     yield;
 }
 
-var {:layer 1, 1} {:linear "mem"} pool: lmap;
+var {:layer 1, 2} {:linear "mem"} pool: lmap;
 var {:layer 0, 1} mem:[int]int;
 var {:layer 0, 1} unallocated:[int]bool;
 
